src/drf/DRF_PF3.v
@@ -113,6 +113,1079 @@ Proof.
       i. ss. eapply List.in_or_app; eauto.
 Qed.
 
+(* Definition self_latest_reseves_loc (mem prom: Memory.t) (loc: Loc.t): Prop := *)
+(*   Memory.latest_reserve loc mem prom. *)
+
+Definition other_latest_reserves (L: Loc.t -> Prop)
+           (mem: Memory.t) (loc: Loc.t) (to: Time.t) (from: Time.t) :=
+  (<<LATEST: to = Memory.max_ts loc mem>>) /\
+  (<<RESERVE: Memory.get loc to mem = Some (from, Message.reserve)>>) /\
+  (<<OTHER: L loc>>)
+.
+
+Definition other_latest_reserves_times (L: Loc.t -> Prop)
+           (mem: Memory.t) (loc: Loc.t) (to: Time.t): Prop :=
+  exists from,
+    (<<RESERVE: other_latest_reserves L mem loc to from>>).
+
+Definition other_caps (L: Loc.t -> Prop)
+           (mem0 mem1: Memory.t) (loc: Loc.t) (to: Time.t) (from: Time.t) :=
+  (<<FULL: Memory.max_full_ts mem0 loc from>>) /\
+  (<<LATEST: exists from0 val released,
+      (<<CAP: caps mem0 mem1 loc to from0 (Message.full val released)>>)>>) /\
+  (<<OTHER: L loc>>)
+.
+
+Definition other_caps_times (L: Loc.t -> Prop)
+           (mem0 mem1: Memory.t) (loc: Loc.t) (to: Time.t) :=
+  exists from,
+    (<<CAP: other_caps L mem0 mem1 loc to from>>).
+
+Definition times_in_memory (mem: Memory.t) (L: Loc.t -> list Time.t): Prop :=
+  forall loc t,
+    (<<SAT: List.In t (L loc)>>) <->
+    (<<INMEMORY:
+       (exists from msg, (<<GET: Memory.get loc t mem = Some (from, msg)>>)) \/
+       (exists to msg, (<<GET: Memory.get loc to mem = Some (t, msg)>>))>>).
+
+Lemma times_in_memory_exists mem
+  :
+    exists l, times_in_memory mem l.
+Proof.
+  hexploit (choice
+              (fun loc tl =>
+                 forall t,
+                   (<<SAT: List.In t tl>>) <->
+                   (<<INMEMORY:
+                      (exists from msg, (<<GET: Memory.get loc t mem = Some (from, msg)>>)) \/
+                      (exists to msg, (<<GET: Memory.get loc to mem = Some (t, msg)>>))>>))); auto.
+  intros loc.
+  hexploit (wf_cell_msgs_exists (mem loc)). i. des.
+  exists ((List.map (fun ftm =>
+                       match ftm with
+                       | (from, _, _) => from
+                       end) l)
+            ++
+            (List.map (fun ftm =>
+                         match ftm with
+                         | (_, to, _) => to
+                         end) l)).
+  i. split; i.
+  - red in H. eapply List.in_app_or in H. des.
+    + eapply List.in_map_iff in H. des.
+      destruct x as [[from to] msg]. clarify.
+      eapply COMPLETE in H0. right. eauto.
+    + eapply List.in_map_iff in H. des.
+      destruct x as [[from to] msg]. clarify.
+      eapply COMPLETE in H0. left. eauto.
+  - eapply List.in_or_app.  des.
+    + right. eapply COMPLETE in GET.
+      eapply List.in_map_iff. esplits; eauto. ss.
+    + left. eapply COMPLETE in GET.
+      eapply List.in_map_iff. esplits; eauto. ss.
+Qed.
+
+Inductive other_collapsing (L: Loc.t -> Prop)
+          (mem: Memory.t): Loc.t -> Time.t -> Time.t -> Prop :=
+| other_collapsing_not_in
+    loc t
+    (NSAT: ~ L loc)
+  :
+    other_collapsing L mem loc t t
+| other_collapsing_in_memory
+    loc t max
+    (SAT: L loc)
+    (FULL: Memory.max_full_ts mem loc max)
+    (TLE: Time.le t max)
+  :
+    other_collapsing L mem loc t t
+| other_collapsing_latest_reserve
+    loc t max
+    (SAT: L loc)
+    (FULL: Memory.max_full_ts mem loc max)
+    (MAX: t = Memory.max_ts loc mem)
+  :
+    other_collapsing L mem loc max t
+| other_collapsing_cap
+    loc t max
+    (SAT: L loc)
+    (FULL: Memory.max_full_ts mem loc max)
+    (CAP: t = Time.incr (Memory.max_ts loc mem))
+  :
+    other_collapsing L mem loc max t
+| other_collapsing_outer_memory
+    loc t max
+    (SAT: L loc)
+    (MAX: max = Memory.max_ts loc mem)
+    (TLE: Time.lt max t)
+  :
+    other_collapsing L mem loc t t
+.
+
+Lemma forget_memory_get P mem0 mem1 loc to msg
+      (FORGET: forget_memory P mem0 mem1)
+      (GET: Memory.get loc to mem0 = Some msg)
+  :
+    (<<NOT: ~ P loc to>>) /\ (<<GET: Memory.get loc to mem1 = Some msg>>).
+Proof.
+  inv FORGET. destruct (classic (P loc to)).
+  - exfalso. rewrite FORGET0 in GET; auto. clarify.
+  - esplits; eauto.
+    rewrite <- COMPLETE; auto.
+Qed.
+
+Lemma caps_get_reserve mem0 prom mem1 loc to from
+      (RESERVE: Memory.reserve_wf prom mem0)
+      (INHABITED: Memory.inhabited mem0)
+      (CLOSED: Memory.closed mem0)
+      (CAP: Memory.cap prom mem0 mem1)
+      (CAPS: caps mem0 mem1 loc to from Message.reserve)
+  :
+    exists from0 to1 msg0 msg1,
+      (<<GET0: Memory.get loc from mem0 = Some (from0, msg0)>>) /\
+      (<<GET1: Memory.get loc to1 mem0 = Some (to, msg1)>>) /\
+      (<<SPACE: forall t (ITV: Interval.mem (from, to) t), ~ covered loc t mem0>>)
+.
+Proof.
+  unfold caps in CAPS. des. inv CAP.
+  exploit COMPLETE; eauto. i. des.
+  set (@cell_elements_least
+         (mem0 loc)
+         (fun t => Time.lt from t)). des.
+  - hexploit (MIDDLE loc f from from0 to0).
+    { econs; eauto. i.
+      destruct (Memory.get loc ts mem0) eqn:GET2; auto. destruct p.
+      exfalso. exploit LEAST.
+      - eapply GET2.
+      - eauto.
+      - i. exploit Memory.get_ts; try apply GET.
+        i. des; clarify.
+        + eapply Time.lt_strorder. eapply TimeFacts.lt_le_lt.
+          * eapply SAT.
+          * eapply Time.bot_spec.
+        + eapply Time.lt_strorder. eapply TimeFacts.le_lt_lt.
+          * etrans.
+            { eapply x1. }
+            { eapply TS2. }
+          * eauto. }
+    { exploit memory_get_from_mon.
+      - eapply x.
+      - eapply GET.
+      - eauto.
+      - i. destruct x2; auto. destruct H. exfalso.
+        exploit memory_get_from_inj.
+        { eapply SOUND. eapply GET. }
+        { eapply GET1. }
+        i. des; clarify.
+        + setoid_rewrite GET0 in GET. clarify.
+        + eapply Time.lt_strorder; eauto. }
+    i. exploit memory_get_from_inj.
+    { eapply H. }
+    { eapply GET1. }
+    i. des; clarify.
+    + esplits; eauto. ii. inv H0.
+      exploit Memory.get_disjoint.
+      * eapply SOUND. eapply GET2.
+      * eapply H.
+      * i. des; clarify. eapply x2; eauto.
+    + specialize (INHABITED loc).
+      eapply SOUND in INHABITED. clarify.
+  - exploit Memory.max_ts_spec.
+    { eapply x. }
+    i. des. destruct MAX.
+    + exfalso. eapply EMPTY; eauto.
+    + unfold Time.eq in *. subst. exploit x0; auto. intros LATEST.
+      exploit Memory.latest_val_exists; eauto. i. des.
+      exploit Memory.max_full_view_exists; eauto. i. des.
+      exploit BACK; eauto. i.
+      exploit memory_get_from_inj.
+      * eapply x1.
+      * eapply GET1.
+      * i. des; clarify.
+        { exfalso. eapply Time.lt_strorder. eapply TimeFacts.lt_le_lt.
+          - eapply Time.incr_spec.
+          - rewrite BOT0. eapply Time.bot_spec. }
+        { erewrite INHABITED in GET0. clarify. }
+Qed.
+
+Definition memory_concrete_le (lhs rhs: Memory.t): Prop :=
+  forall loc to from val released
+         (GET: Memory.get loc to lhs = Some (from, Message.full val released)),
+    Memory.get loc to rhs = Some (from, Message.full val released).
+
+Lemma memory_concrete_le_le
+  :
+    Memory.le <2= memory_concrete_le.
+Proof.
+  ii. eauto.
+Qed.
+Hint Resolve memory_concrete_le_le.
+
+Lemma memory_concrete_le_closed_timemap tm mem0 mem1
+      (MLE: memory_concrete_le mem0 mem1)
+      (TM: Memory.closed_timemap tm mem0)
+  :
+    Memory.closed_timemap tm mem1.
+Proof.
+  ii. hexploit (TM loc). i. des.
+  esplits; eauto.
+Qed.
+
+Lemma memory_concrete_le_closed_view vw mem0 mem1
+      (MLE: memory_concrete_le mem0 mem1)
+      (VW: Memory.closed_view vw mem0)
+  :
+    Memory.closed_view vw mem1.
+Proof.
+  inv VW. econs.
+  - eapply memory_concrete_le_closed_timemap; eauto.
+  - eapply memory_concrete_le_closed_timemap; eauto.
+Qed.
+
+Lemma memory_concrete_le_closed_opt_view vw mem0 mem1
+      (MLE: memory_concrete_le mem0 mem1)
+      (VW: Memory.closed_opt_view vw mem0)
+  :
+    Memory.closed_opt_view vw mem1.
+Proof.
+  inv VW; econs.
+  eapply memory_concrete_le_closed_view; eauto.
+Qed.
+
+Lemma memory_concrete_le_closed_msg msg mem0 mem1
+      (MLE: memory_concrete_le mem0 mem1)
+      (MSG: Memory.closed_message msg mem0)
+  :
+    Memory.closed_message msg mem1.
+Proof.
+  inv MSG; econs.
+  eapply memory_concrete_le_closed_opt_view; eauto.
+Qed.
+
+Lemma memory_concrete_le_closed_tview vw mem0 mem1
+      (MLE: memory_concrete_le mem0 mem1)
+      (VW: TView.closed vw mem0)
+  :
+    TView.closed vw mem1.
+Proof.
+  inv VW. econs.
+  - i. eapply memory_concrete_le_closed_view; eauto.
+  - eapply memory_concrete_le_closed_view; eauto.
+  - eapply memory_concrete_le_closed_view; eauto.
+Qed.
+
+Lemma memory_concrete_le_reserve_wf prom mem0 mem1
+      (MLE: memory_concrete_le mem0 mem1)
+      (RESERVE: Memory.reserve_wf prom mem0)
+  :
+    Memory.reserve_wf prom mem1.
+Proof.
+  ii. eapply RESERVE in GET. des.
+  esplits; eauto.
+Qed.
+
+Lemma memory_concrete_le_local_wf lc mem0 mem1
+      (MLE: memory_concrete_le mem0 mem1)
+      (PROM: Memory.le (Local.promises lc) mem1)
+      (LOCAL: Local.wf lc mem0)
+  :
+    Local.wf lc mem1.
+Proof.
+  inv LOCAL. econs; eauto.
+  - eapply memory_concrete_le_closed_tview; eauto.
+  - eapply memory_concrete_le_reserve_wf; eauto.
+Qed.
+
+Lemma partial_cap_closed prom mem0 mem1 mem2
+      (MLE: Memory.le prom mem0)
+      (CLOSED: Memory.closed mem0)
+      (RESERVEWF: Memory.reserve_wf prom mem0)
+      (INHABITED: Memory.inhabited mem0)
+      (CAP: Memory.cap prom mem0 mem2)
+      (MLE0: Memory.le mem0 mem1)
+      (MLE1: Memory.le mem1 mem2)
+  :
+    Memory.closed mem1.
+Proof.
+  exploit Memory.max_full_timemap_exists; eauto. intros [tm MAX].
+  inv CLOSED. econs; eauto.
+  i. destruct (Memory.get loc to mem0) as [[from0 msg0]|] eqn:GET.
+  - dup GET. eapply MLE0 in GET. clarify.
+    eapply CLOSED0 in GET0. des. esplits; eauto.
+    eapply memory_concrete_le_closed_msg; eauto.
+  - destruct msg.
+    + eapply MLE1 in MSG.
+      exploit caps_max_view; eauto.
+      * econs; eauto.
+      * i. des; clarify. esplits; eauto.
+        { econs; eauto. econs; eauto. econs. refl. }
+        { econs; eauto. ss. transitivity (Memory.max_ts loc mem0).
+          - specialize (MAX loc). inv MAX. des.
+            eapply Memory.max_ts_spec in GET0. des. eauto.
+          - left. eapply Time.incr_spec. }
+        { eapply memory_concrete_le_closed_msg; eauto.
+          econs. econs. econs.
+          - eapply Memory.max_full_timemap_closed; eauto.
+          - eapply Memory.max_full_timemap_closed; eauto. }
+    + esplits; eauto. econs.
+Qed.
+
+Lemma other_caps_forget_le
+      mem0 mem1 mem2 prom (L: Loc.t -> Prop)
+      (CAP: Memory.cap prom mem0 mem2)
+      (FORGET: forget_memory (other_latest_reserves_times L mem0 \2/ other_caps_times L mem0 mem1) mem1 mem2)
+  :
+    memory_concrete_le mem0 mem1.
+Proof.
+  inv FORGET. ii.
+  erewrite COMPLETE.
+  - eapply Memory.cap_le in CAP; eauto. refl.
+  - ii. des.
+    + unfold other_latest_reserves_times in *. des.
+      inv RESERVE. des. clarify.
+    + unfold other_caps_times in *. des.
+      inv CAP0. des. unfold caps in CAP0. des. clarify.
+Qed.
+
+Lemma other_caps_forget_prom_le
+      mem0 mem1 mem2 prom (L: Loc.t -> Prop)
+      (OTHERS: forall loc (SAT: L loc), Memory.latest_reserve loc prom mem0)
+      (MLE: Memory.le prom mem0)
+      (CLOSED: Memory.closed mem0)
+      (RESERVEWF: Memory.reserve_wf prom mem0)
+      (INHABITED: Memory.inhabited mem0)
+      (CAP: Memory.cap prom mem0 mem2)
+      (FORGET: forget_memory (other_latest_reserves_times L mem0 \2/ other_caps_times L mem0 mem1) mem1 mem2)
+  :
+    Memory.le prom mem1.
+Proof.
+  inv FORGET. ii.
+  erewrite COMPLETE.
+  - eapply Memory.cap_le in CAP; eauto.
+  - ii. des.
+    + unfold other_latest_reserves_times in *. des.
+      inv RESERVE. des. clarify.
+      dup LHS. eapply MLE in LHS0. clarify.
+      eapply OTHERS in OTHER. unfold Memory.latest_reserve in OTHER.
+      rewrite LHS in *. clarify.
+    + unfold other_caps_times in *. des.
+      inv CAP0. des. unfold caps in CAP0. des.
+      eapply MLE in LHS; eauto. clarify.
+Qed.
+
+Lemma identity_mapped_view tm maxmap (f: Loc.t -> Time.t -> Time.t -> Prop)
+      (TM: TimeMap.le tm maxmap)
+      (IDENT: forall loc ts (TS: Time.le ts (maxmap loc)), f loc ts ts)
+  :
+    timemap_map f tm tm.
+Proof.
+  ii. eapply IDENT; eauto.
+Qed.
+
+Lemma other_collapsing_ident L mem loc maxts ts
+      (MAX: Memory.max_full_ts mem loc maxts)
+      (TS: Time.le ts maxts)
+  :
+    (other_collapsing L mem) loc ts ts.
+Proof.
+  i. destruct (classic (L loc)).
+  - econs 2; eauto.
+  - econs 1; eauto.
+Qed.
+
+Definition memory_reserve_wf mem := Memory.reserve_wf mem mem.
+
+Lemma memory_reserve_wf_promise
+      prom0 mem0 loc from to msg prom1 mem1 kind
+      (PROMISE: Memory.promise prom0 mem0 loc from to msg prom1 mem1 kind)
+      (RESERVE: memory_reserve_wf mem0)
+  :
+    memory_reserve_wf mem1.
+Proof.
+  inv PROMISE.
+  - ii. erewrite Memory.add_o in GET; eauto. des_ifs.
+    + ss; des; clarify. exploit RESERVE0; eauto.
+      i. des. eapply Memory.add_get1 in x; eauto.
+    + eapply RESERVE in GET; eauto. clear o. des.
+      eapply Memory.add_get1 in GET; eauto.
+  - ii. des. clarify. erewrite Memory.split_o in GET; eauto. des_ifs.
+    + ss; des; clarify. eapply Memory.split_get0 in MEM. des.
+      esplits; eauto.
+    + eapply RESERVE in GET; eauto. clear o o0. des.
+      eapply Memory.split_get1 in GET; eauto. des. esplits; eauto.
+  - ii. erewrite Memory.lower_o in GET; eauto. des_ifs.
+    + ss; des; clarify. inv MEM. inv LOWER. inv MSG_LE.
+    + eapply RESERVE in GET; eauto. clear o. des.
+      eapply Memory.lower_get1 in GET; eauto. des.
+      inv MSG_LE. esplits; eauto.
+  - ii. erewrite Memory.remove_o in GET; eauto. des_ifs. guardH o.
+    dup MEM. eapply Memory.remove_get0 in MEM0. des.
+    eapply RESERVE in GET; eauto. des. dup GET.
+    eapply Memory.remove_get1 in GET2; eauto. ss. des; clarify.
+    esplits; eauto.
+Qed.
+
+Lemma memory_reserve_wf_tstep lang (th0 th1: Thread.t lang) tf e
+      (RESERVE: memory_reserve_wf th0.(Thread.memory))
+      (STEP: Thread.step tf e th0 th1)
+  :
+    memory_reserve_wf th1.(Thread.memory).
+Proof.
+  inv STEP; inv STEP0; ss.
+  - inv LOCAL. eapply memory_reserve_wf_promise; eauto.
+  - inv LOCAL; eauto.
+    + inv LOCAL0. inv WRITE.
+      eapply memory_reserve_wf_promise; eauto.
+    + inv LOCAL1. inv LOCAL2. inv WRITE.
+      eapply memory_reserve_wf_promise; eauto.
+Qed.
+
+Lemma memory_reserve_wf_tsteps lang (th0 th1: Thread.t lang)
+      (RESERVE: memory_reserve_wf th0.(Thread.memory))
+      (STEP: rtc (tau (@Thread.step_allpf lang)) th0 th1)
+  :
+    memory_reserve_wf th1.(Thread.memory).
+Proof.
+  ginduction STEP; eauto.
+  i. eapply IHSTEP; eauto. inv H. inv TSTEP.
+  eapply memory_reserve_wf_tstep; eauto.
+Qed.
+
+Lemma memory_reserve_wf_init
+  :
+    memory_reserve_wf Memory.init.
+Proof.
+  ii. unfold Memory.get, Memory.init in *. ss.
+  rewrite Cell.init_get in GET. des_ifs.
+Qed.
+
+Lemma memory_reserve_wf_configuration_step c0 c1 e tid
+      (RESERVE: memory_reserve_wf c0.(Configuration.memory))
+      (STEP: Configuration.step e tid c0 c1)
+  :
+    memory_reserve_wf c1.(Configuration.memory).
+Proof.
+  eapply configuration_step_equivalent in STEP. inv STEP. ss.
+  eapply memory_reserve_wf_tstep in STEP0; eauto.
+  eapply memory_reserve_wf_tsteps in STEPS; eauto.
+Qed.
+
+Lemma not_latest_reserve_le_max_full_ts loc mem ts to from msg
+      (RESERVEWF : memory_reserve_wf mem)
+      (INHABITED : Memory.inhabited mem)
+      (MAX : Memory.max_full_ts mem loc ts)
+      (GET: Memory.get loc to mem = Some (from, msg))
+  :
+    (<<TLE: Time.le to ts>>) \/
+    ((<<TO: to = Memory.max_ts loc mem>>) /\
+     (<<FROM: from = ts>>) /\
+     (<<MSG: msg = Message.reserve>>)).
+Proof.
+  inv MAX. des.
+  destruct msg.
+  - left. eapply MAX0; eauto.
+  - exploit RESERVEWF; eauto. i. des.
+    destruct (TimeFacts.le_lt_dec to ts); auto.
+    dup x. eapply MAX0 in x; eauto. destruct x.
+    + exfalso. exploit memory_get_from_mon.
+      { eapply GET0. }
+      { eapply GET. }
+      { auto. }
+      i. eapply Time.lt_strorder. eapply TimeFacts.le_lt_lt.
+      * eapply x1.
+      * eapply H.
+    + unfold Time.eq in *. subst. right. esplits; eauto.
+      setoid_rewrite GET0 in x0. clarify.
+      dup GET. eapply Memory.max_ts_spec in GET1. des.
+      destruct MAX; auto. exfalso.
+      destruct msg.
+      * eapply MAX0 in GET2. eapply Time.lt_strorder.
+        eapply TimeFacts.lt_le_lt.
+        { etrans.
+          - eapply l.
+          - eapply H. }
+        { eauto. }
+      * dup GET2. eapply RESERVEWF in GET2. des.
+        eapply MAX0 in GET2.
+        exploit memory_get_from_mon.
+        { eapply GET. }
+        { eapply GET1. }
+        { eapply H. }
+        i. eapply Time.lt_strorder.
+        eapply TimeFacts.lt_le_lt.
+        { eapply l. }
+        { etrans.
+          - eapply x0.
+          - eapply Memory.get_ts in GET1. des; clarify. }
+Qed.
+
+Lemma max_full_ts_le_max_ts mem loc ts
+      (MAX: Memory.max_full_ts mem loc ts)
+  :
+    Time.le ts (Memory.max_ts loc mem).
+Proof.
+  inv MAX. des.
+  eapply Memory.max_ts_spec in GET. des; auto.
+Qed.
+
+Lemma max_full_ts_max_ts loc mem ts
+      (RESERVEWF : memory_reserve_wf mem)
+      (INHABITED : Memory.inhabited mem)
+      (MAX : Memory.max_full_ts mem loc ts)
+  :
+    (<<FULL: ts = Memory.max_ts loc mem>>) \/
+    ((<<TLT: Time.lt ts (Memory.max_ts loc mem)>>) /\
+     (<<GET: Memory.get loc (Memory.max_ts loc mem) mem = Some (ts, Message.reserve)>>)).
+Proof.
+  dup MAX. inv MAX. des.
+  eapply Memory.max_ts_spec in GET. des.
+  dup GET0. eapply not_latest_reserve_le_max_full_ts in GET0; eauto.
+  des; clarify.
+  - left. eapply TimeFacts.antisym; eauto.
+  - right. split; eauto. dup GET1.
+    eapply memory_get_ts_strong in GET1. des; clarify.
+    erewrite GET2 in *.
+    erewrite INHABITED in GET0. clarify.
+Qed.
+
+Lemma other_collapsing_ident2 L mem maxts loc ts fts
+      (MAX: Memory.max_full_ts mem loc maxts)
+      (TS: Time.le fts maxts)
+      (MAP: (other_collapsing L mem) loc ts fts)
+  :
+    ts = fts.
+Proof.
+  inv MAP; eauto.
+  - exploit Memory.max_full_ts_inj.
+    { eapply FULL. }
+    { eapply MAX. }
+    i. clarify. eapply TimeFacts.antisym; auto.
+    eapply max_full_ts_le_max_ts in FULL; auto.
+  - exfalso. eapply max_full_ts_le_max_ts in FULL. exfalso.
+    eapply Time.lt_strorder. eapply TimeFacts.lt_le_lt.
+    + eapply DenseOrder.DenseOrder.incr_spec.
+    + etrans.
+      * eapply TS.
+      * eapply max_full_ts_le_max_ts; eauto.
+Qed.
+
+Lemma other_collapsing_ident3 L mem maxts loc ts fts
+      (RESERVEWF : memory_reserve_wf mem)
+      (INHABITED : Memory.inhabited mem)
+      (MAX: Memory.max_full_ts mem loc maxts)
+      (TS: Time.lt ts maxts)
+      (MAP: (other_collapsing L mem) loc ts fts)
+  :
+    ts = fts.
+Proof.
+  inv MAP; eauto.
+  - exploit Memory.max_full_ts_inj.
+    { eapply FULL. }
+    { eapply MAX. }
+    i. clarify. exfalso. eapply Time.lt_strorder; eauto.
+  - exploit Memory.max_full_ts_inj.
+    { eapply FULL. }
+    { eapply MAX. }
+    i. clarify. exfalso. eapply Time.lt_strorder; eauto.
+Qed.
+
+Lemma other_collapsing_timemap L mem tm
+      (INHABITED: Memory.inhabited mem)
+      (TM: Memory.closed_timemap tm mem)
+  :
+    timemap_map (other_collapsing L mem) tm tm.
+Proof.
+  exploit Memory.max_full_timemap_exists; eauto. intros [maxmap MAX].
+  eapply identity_mapped_view.
+  - eapply Memory.max_full_timemap_spec; eauto.
+  - i. eapply other_collapsing_ident; eauto.
+Qed.
+
+Lemma other_collapsing_view L mem vw
+      (INHABITED: Memory.inhabited mem)
+      (VW: Memory.closed_view vw mem)
+  :
+    view_map (other_collapsing L mem) vw vw.
+Proof.
+  inv VW. econs.
+  - eapply other_collapsing_timemap; eauto.
+  - eapply other_collapsing_timemap; eauto.
+Qed.
+
+Lemma other_collapsing_opt_view L mem vw
+      (INHABITED: Memory.inhabited mem)
+      (VW: Memory.closed_opt_view vw mem)
+  :
+    opt_view_map (other_collapsing L mem) vw vw.
+Proof.
+  inv VW; econs.
+  eapply other_collapsing_view; eauto.
+Qed.
+
+Lemma other_collapsing_message L mem msg
+      (INHABITED: Memory.inhabited mem)
+      (MSG: Memory.closed_message msg mem)
+  :
+    msg_map (other_collapsing L mem) msg msg.
+Proof.
+  inv MSG; econs.
+  eapply other_collapsing_opt_view; eauto.
+Qed.
+
+Lemma other_collapsing_tview L mem vw
+      (INHABITED: Memory.inhabited mem)
+      (VW: TView.closed vw mem)
+  :
+    tview_map (other_collapsing L mem) vw vw.
+Proof.
+  inv VW. econs.
+  - i. eapply other_collapsing_view; eauto.
+  - eapply other_collapsing_view; eauto.
+  - eapply other_collapsing_view; eauto.
+Qed.
+
+
+Lemma other_collapsing_promises (L: Loc.t -> Prop) mem prom
+      (MLE: Memory.le prom mem)
+      (CLOSED: Memory.closed mem)
+      (RESERVEWF: memory_reserve_wf mem)
+      (INHABITED: Memory.inhabited mem)
+      (OTHERS: forall loc (SAT: L loc), Memory.latest_reserve loc prom mem)
+  :
+    promises_map (other_collapsing L mem) prom prom.
+Proof.
+  exploit Memory.max_full_timemap_exists; eauto. intros [tm MAX].
+  dup CLOSED. inv CLOSED0. econs.
+  - i. dup GET. eapply MLE in GET0. eapply CLOSED1 in GET0. des.
+    exists to, from, msg.
+    destruct (classic (L loc)).
+    + dup GET. eapply MLE in GET0.
+      eapply not_latest_reserve_le_max_full_ts in GET0; eauto.
+      eapply or_strengthen in GET0. des; clarify.
+      * esplits; eauto.
+        { ii. unfold collapsed in *. des.
+          eapply other_collapsing_ident3 in MAP0; eauto; cycle 1.
+          { eapply TimeFacts.lt_le_lt; eauto. } clarify.
+          assert (TO: to = ft).
+          { destruct TLE.
+            - eapply other_collapsing_ident3 in MAP1; eauto.
+            - unfold Time.eq in *. clarify. inv MAP1; clarify.
+              + exfalso. eapply Time.lt_strorder.
+                eapply TimeFacts.lt_le_lt.
+                * eapply TLE0.
+                * eapply max_full_ts_le_max_ts; eauto.
+              + exfalso. eapply Time.lt_strorder.
+                eapply TimeFacts.lt_le_lt.
+                * etrans.
+                  { eapply Time.incr_spec. }
+                  { eapply TLE0. }
+                * eapply max_full_ts_le_max_ts; eauto. }
+          clarify. eapply Time.lt_strorder; eauto. }
+        { econs 2; eauto. }
+        { eapply other_collapsing_message; eauto. }
+      * exfalso. exploit OTHERS; eauto.
+        unfold Memory.latest_reserve. rewrite GET. auto.
+    + splits; auto.
+      * ii. unfold collapsed in *. des.
+        inv MAP0; clarify. inv MAP1; clarify.
+        eapply Time.lt_strorder. eauto.
+      * econs 1; eauto.
+      * eapply other_collapsing_message; eauto.
+
+  - i. exists fto, ffrom, fmsg.
+    destruct (classic (L loc)).
+    + dup GET. eapply MLE in GET.
+      eapply not_latest_reserve_le_max_full_ts in GET; eauto.
+      des; clarify.
+      * splits; auto.
+        { eapply other_collapsing_ident; eauto. }
+        { eapply other_collapsing_ident; eauto.
+          etrans; eauto.
+          eapply memory_get_ts_strong in GET0. des; clarify.
+          { refl. }
+          { left. auto. } }
+      * exfalso. exploit OTHERS; eauto.
+        unfold Memory.latest_reserve. rewrite GET0. auto.
+    + splits; auto.
+      * econs 1; eauto.
+      * econs 1; eauto.
+Qed.
+
+
+
+Lemma other_collapsing_memory
+      mem0 mem1 mem2 prom (L: Loc.t -> Prop)
+      (MLE: Memory.le prom mem0)
+      (CLOSED: Memory.closed mem0)
+      (RESERVEWF: Memory.reserve_wf prom mem0)
+      (INHABITED: Memory.inhabited mem0)
+      (OTHERS: forall loc (SAT: L loc), Memory.latest_reserve loc prom mem0)
+      (CAP: Memory.cap prom mem0 mem1)
+      (FORGET: forget_memory (other_latest_reserves_times L mem0 \2/ other_caps_times L mem0 mem1) mem2 mem1)
+  :
+    memory_map (other_collapsing L mem0) mem2 mem1.
+Proof.
+  exploit Memory.max_full_timemap_exists; eauto. intros [tm MAX].
+  dup CLOSED. inv CLOSED0. econs.
+  - i. destruct (classic (L loc)).
+    + dup GET. eapply forget_memory_get in GET0; eauto. des.
+
+
+      dup FORGET.
+
+      admit.
+
+    + exists to, from, msg, msg. esplits; eauto.
+      * econs 1; eauto.
+      * eapply other_collapsing_message; eauto.
+        eapply CLOSED1.
+
+               econs 1; eauto.
+
+
+
+    admit.
+
+  - i. exists fto, ffrom, fmsg.
+    destruct (classic (L loc)).
+    + splits; auto.
+      * econs 2; eauto.
+      * inv FORGET. erewrite COMPLETE; eauto.
+        ii. des.
+        { unfold other_latest_reserves_times, other_latest_reserves in H0.
+          des. clarify. }
+        { unfold other_caps_times, other_caps in H0.
+          des. clarify. }
+      * econs 1; eauto.
+
+
+      admit.
+    + splits; auto.
+      * econs 1; eauto.
+      * inv FORGET. erewrite COMPLETE; eauto.
+        ii. des.
+        { unfold other_latest_reserves_times, other_latest_reserves in H0.
+          des. clarify. }
+        { unfold other_caps_times, other_caps in H0.
+          des. clarify. }
+      * econs 1; eauto.
+
+
+        econs 1; eauto.
+
+
+    + dup GET. eapply MLE in GET.
+      eapply not_latest_reserve_le_max_full_ts in GET; eauto.
+      des; clarify.
+      * splits; auto.
+        { eapply other_collapsing_ident; eauto. }
+        { eapply other_collapsing_ident; eauto.
+          etrans; eauto.
+          eapply memory_get_ts_strong in GET0. des; clarify.
+          { refl. }
+          { left. auto. } }
+      * exfalso. exploit OTHERS; eauto.
+        unfold Memory.latest_reserve. rewrite GET0. auto.
+    + splits; auto.
+      * econs 1; eauto.
+      * econs 1; eauto.
+
+
+  - i. dup GET. eapply CLOSED1 in GET0. des.
+    exists to, from, msg.
+    destruct (classic (L loc)).
+    + dup GET. eapply MLE in GET0.
+      eapply not_latest_reserve_le_max_full_ts in GET0; eauto.
+      eapply or_strengthen in GET0. des; clarify.
+      * esplits; eauto.
+        { ii. unfold collapsed in *. des.
+          eapply other_collapsing_ident3 in MAP0; eauto; cycle 1.
+          { eapply TimeFacts.lt_le_lt; eauto. } clarify.
+          assert (TO: to = ft).
+          { destruct TLE.
+            - eapply other_collapsing_ident3 in MAP1; eauto.
+            - unfold Time.eq in *. clarify. inv MAP1; clarify.
+              + exfalso. eapply Time.lt_strorder.
+                eapply TimeFacts.lt_le_lt.
+                * eapply TLE0.
+                * eapply max_full_ts_le_max_ts; eauto.
+              + exfalso. eapply Time.lt_strorder.
+                eapply TimeFacts.lt_le_lt.
+                * etrans.
+                  { eapply Time.incr_spec. }
+                  { eapply TLE0. }
+                * eapply max_full_ts_le_max_ts; eauto. }
+          clarify. eapply Time.lt_strorder; eauto. }
+        { econs 2; eauto. }
+        { eapply other_collapsing_message; eauto. }
+      * exfalso. exploit OTHERS; eauto.
+        unfold Memory.latest_reserve. rewrite GET. auto.
+    + splits; auto.
+      * ii. unfold collapsed in *. des.
+        inv MAP0; clarify. inv MAP1; clarify.
+        eapply Time.lt_strorder. eauto.
+      * econs 1; eauto.
+      * eapply other_collapsing_message; eauto.
+
+  - i. exists fto, ffrom, fmsg.
+    destruct (classic (L loc)).
+    + dup GET. eapply MLE in GET.
+      eapply not_latest_reserve_le_max_full_ts in GET; eauto.
+      des; clarify.
+      * splits; auto.
+        { eapply other_collapsing_ident; eauto. }
+        { eapply other_collapsing_ident; eauto.
+          etrans; eauto.
+          eapply memory_get_ts_strong in GET0. des; clarify.
+          { refl. }
+          { left. auto. } }
+      * exfalso. exploit OTHERS; eauto.
+        unfold Memory.latest_reserve. rewrite GET0. auto.
+    + splits; auto.
+      * econs 1; eauto.
+      * econs 1; eauto.
+Qed.
+
+
+  exploit Memory.max_full_timemap_exists; eauto. intros [tm MAX].
+  dup FORGET. inv FORGET. econs.
+  - i. dup GET. eapply forget_memory_get in GET; eauto.
+    ss. des. apply not_or_and in NOT. des.
+    exists to, from, msg, msg. esplits.
+    + destruct (classic (L loc)).
+      * econs 2; eauto. specialize (MAX loc). inv MAX.
+        destruct msg as [val released|].
+        { eapply MAX0; eauto.
+
+
+        exploit Memory.max_full_ts_exists; eauto.
+        instantiate (1:=loc). i. des. econs 2; eauto. inv x0.
+        destruct msg as [val released|].
+        {
+
+          eapply caps_max_view in
+
+
+          admit
+
+          eapply MAX in GET1.
+
+        inv x0.
+
+
+
+        x
+
+        { eauto
+
+        econs 2; eauto.
+
+
+        admit.
+      * econs 1; eauto.
+    + destruct msg; econs.
+      destruct released; econs.
+
+               econs.
+
+
+
+              r
+    ss. des.
+    destruct (classic (other_latest_reserves_times L mem0 loc to \/ other_caps_times L mem0 mem1 loc to)); cycle 1.
+
+
+
+
+    forget_memory
+
+
+    Memory.cap
+
+->
+
+
+Definition other_latest_reserves_times (L: Loc.t -> Prop)
+           (mem: Memory.t) (loc: Loc.t) (to: Time.t) :=
+  exists from,
+    (<<RESERVE: other_latest_reserves L mem loc to from>>).
+
+Definition other_caps_times (L: Loc.t -> Prop)
+           (mem0 mem1: Memory.t) (loc: Loc.t) (to: Time.t) :=
+  exists from,
+    (<<CAP: other_caps L mem0 mem1 loc to from>>).
+
+
+
+Inductive other_collapsing (L: Loc.t -> Prop)
+          (mem0 mem1: Memory.t): Loc.t -> Time.t -> Time.t -> Prop :=
+| other_collapsing_not_in
+    loc t
+    (NSAT: ~ L loc)
+  :
+    other_collapsing L mem0 mem1 loc t t
+| other_collapsing_in_memory
+    loc t max
+    (SAT: L loc)
+    (MAX: Memory.max_full_ts mem0 loc max)
+    (TLE: Time.le t max)
+  :
+    other_collapsing L mem0 mem1 loc t t
+| other_collapsing_in_memory
+    loc t max
+    (SAT: L loc)
+    (MAX: Memory.max_full_ts mem0 loc max)
+    (TLE: Time.le t max)
+  :
+    other_collapsing L mem0 mem1 loc t t
+.
+
+
+
+
+           Variable f: Loc.t -> Time.t -> Time.t -> Prop.
+  Hypothesis map_le:
+    forall loc t0 t1 ft0 ft1
+           (MAP0: f loc t0 ft0)
+           (MAP1: f loc t1 ft1),
+      Time.le t0 t1 -> Time.le ft0 ft1.
+  Hypothesis map_bot:
+    forall loc,
+      f loc Time.bot Time.bot.
+  Hypothesis map_eq:
+    forall loc to ft0 ft1
+           (MAP0: f loc to ft0)
+           (MAP1: f loc to ft1),
+      ft0 = ft1.
+
+
+
+
+
+Definition other_caps (L: Loc.t -> Prop)
+           (mem0 mem1: Memory.t) (loc: Loc.t) (to: Time.t) (from: Time.t) :=
+  (<<FULL: Memory.max_full_ts mem0 loc from>>) /\
+  (<<LATEST: exists from0 val released,
+      (<<CAP: caps mem0 mem1 loc to from0 (Message.full val released)>>)>>) /\
+  (<<OTHER: L loc>>)
+.
+
+
+
+
+  Lemma cell_finite_sound_exists c
+    :
+      exists dom,
+        (<<COMPLETE: forall to,
+            (List.In to dom <-> exists from msg,
+                (<<GET: Cell.get to c = Some (from, msg)>>))>>).
+
+
+
+ (mem0 prom : Memory.t) (l : Loc.t) (t from : Time.t) (msg : Message.t)
+
+
+  (<<LATEST: to = Memory.max_ts loc mem>>) /\
+  (<<RESERVE: exists from, (<<GET: Memory.get loc to mem = Some (from, Message.reserve)>>)>>) /\
+  (<<OTHER: L loc>>)
+.
+
+Memory.max_full_ts
+
+Memory.get_
+
+     Memory.get loc (Memory.max_ts loc mem) promises>>
+  (<<LATEST: Memory.get loc (Memory.max_ts loc mem) promises>>
+
+
+
+  forall mem1 (CAP: Memory.cap prom mem0 mem1),
+    (<<GET0: Memory.get l t mem0 = None>>) /\
+    (<<GET1: Memory.get l t mem1 = Some (from, msg)>>).
+
+Memory.cap
+
+                (forall (loc : Loc.t) (val : Const.t) (view : View.t),
+                 Memory.latest_reserve loc promises mem1 ->
+                 Memory.latest_val loc mem1 val ->
+                 Memory.max_full_view mem1 view ->
+                 Memory.get loc (Time.incr (Memory.max_ts loc mem1)) mem2 =
+                 Some (Memory.max_ts loc mem1, Message.full val (Some view))) ->
+
+
+Definition caps (mem0 prom : Memory.t) (l : Loc.t) (t from : Time.t) (msg : Message.t) :=
+  forall mem1 (CAP: Memory.cap prom mem0 mem1),
+    (<<GET0: Memory.get l t mem0 = None>>) /\
+    (<<GET1: Memory.get l t mem1 = Some (from, msg)>>).
+
+Definition partiral_cap (L: Loc.t -> Prop)
+      prom mem1 mem2
+
+
+
+
+Memory.cap
+
+Lemma collapsing_other_cap
+      (
+
+
+
+
+
+
+Inductive shifted_map mlast mcert
+          (updates: Loc.t -> Prop)
+          (sky gap: TimeMap.t)
+          (f: Loc.t -> Time.t -> Time.t): Prop :=
+| shifted_map_intro
+    (PRSV: map_preserving (times_in_memory mcert) f)
+    (SAME: forall l t (TLE: Time.le t (Memory.max_ts l mlast)),
+        f l t = t)
+    (INGAP: forall l t (TLT: Time.lt (Memory.max_ts l mcert) t),
+        Time.lt (f l t) (gap l))
+    (AFTERSKY: forall l t (TLT: Time.lt (Memory.max_ts l mcert) t),
+        Time.lt (sky l) (f l t))
+.
+
+Lemma shifted_map_exists mlast mcert updates
+      (MLE: Memory.le mlast mcert)
+      (sky gap: TimeMap.t)
+      (SKY: forall l, Time.lt (Memory.max_ts l mlast) (sky l))
+      (GAP: forall l, Time.lt (Memory.max_ts l mlast) (gap l))
+  :
+    exists f, (<<SHIFTED: shifted_map mlast mcert updates sky gap f>>).
+Proof.
+  (* may be very hard... *)
+Admitted.
+
+Lemma shifted_map_preserving_last_mem  mlast mcert updates sky gap f
+      (CLOSED: Memory.closed mlast)
+      (SHIFTED: shifted_map mlast mcert updates sky gap f)
+  :
+    memory_map f mlast mlast.
+Proof.
+  inv SHIFTED. inv PRSV. econs; i.
+  - exploit Memory.max_ts_spec; eauto. i. des.
+    repeat erewrite SAME; eauto.
+    + rewrite GET. unfold msg_map. des_ifs. repeat f_equal.
+      inv CLOSED. exploit CLOSED0; try apply GET; eauto. i. des.
+      inv MSG_CLOSED. inv CLOSED; ss. f_equal.
+      destruct view. inv CLOSED1. unfold view_map, timemap_map. ss. f_equal.
+      * extensionality l. erewrite SAME; auto.
+        specialize (PLN l). des.
+        exploit Memory.max_ts_spec; eauto. i. des. auto.
+      * extensionality l. erewrite SAME; auto.
+        specialize (RLX l). des.
+        exploit Memory.max_ts_spec; eauto. i. des. auto.
+    + exploit Memory.get_ts; try apply GET; eauto. i. des.
+      * clarify.
+      * left. eapply TimeFacts.lt_le_lt; eauto.
+  - destruct msg_src as [from msg]. exploit Memory.max_ts_spec; eauto. i. des.
+    esplits.
+    + erewrite SAME; eauto.
+    + eauto.
+Qed.
 
 
 Inductive diff_after_promises (prom mem0 mem1: Memory.t)
